steel/formats/aux/Zeta.Formats.Aux.External.fsti
@@ -1,6 +1,6 @@
 module Zeta.Formats.Aux.External
 
 val significant_digits_t: eqtype
-val significant_digits_st_t: eqtype
+val internal_key: eqtype
 val application_key: eqtype
 val application_value: eqtype
