steel/formats/spec/Zeta.Formats.Aux.Application_key.fst
@@ -1,0 +1,31 @@
+module Zeta.Formats.Aux.Application_key
+
+friend Zeta.Formats.Aux.External
+open Zeta.Steel.ApplicationTypes
+open Zeta.Formats.Lib
+
+let application_key_parser =
+  parser_intro application_key spec_parser_key spec_serializer_key spec_parser_key_injective spec_parser_key_strong_prefix 0 2040 serialized_key_length;
+  spec_parser_key
+
+let application_key_serializer =
+  spec_serializer_key
+
+let application_key_bytesize x = Seq.length (spec_serializer_key x)
+
+let application_key_bytesize_eq x = ()
+
+assume val application_key_parser32': LS.parser32 application_key_parser
+let application_key_parser32 = application_key_parser32'
+
+assume val application_key_serializer32': LS.serializer32 application_key_serializer
+let application_key_serializer32 = application_key_serializer32'
+
+assume val application_key_size32': LS.size32 application_key_serializer
+let application_key_size32 = application_key_size32'
+
+assume val application_key_validator': LL.validator application_key_parser
+let application_key_validator = application_key_validator'
+
+assume val application_key_jumper': LL.jumper application_key_parser
+let application_key_jumper = application_key_jumper'
