steel/formats/spec/Zeta.Formats.Aux.External.fst
@@ -1,0 +1,6 @@
+module Zeta.Formats.Aux.External
+
+let significant_digits_t = Zeta.Steel.LogEntry.Types.significant_digits_t
+let internal_key = Zeta.Steel.LogEntry.Types.internal_key
+let application_key = Zeta.Steel.ApplicationTypes.key_type
+let application_value = Zeta.Steel.ApplicationTypes.value_type
