steel/formats/spec/Zeta.Formats.Lib.fst
@@ -1,0 +1,107 @@
+module Zeta.Formats.Lib
+
+val classical_forall_intro_2_requires
+      (#a: Type)
+      (#b: (a -> Type))
+      (#p #q: (x: a -> b x -> GTot Type0))
+      ($u: (x: a -> y: b x -> Lemma (requires (p x y)) (ensures (q x y))))
+    : Lemma (forall (x: a) (y: b x). p x y ==> q x y)
+
+let classical_forall_intro_2_requires
+  #a #b #p #q u
+= let phi (x: a) (y: b x) : Lemma
+    (p x y ==> q x y)
+  = Classical.move_requires (u x) y
+  in
+  Classical.forall_intro_2 phi
+
+open LowParse.Spec.Base
+
+module P = Zeta.Steel.Parser
+
+// TODO: move to LowParse.Spec.Base
+let parser_injective_intro
+  (#t: Type)
+  (p: bare_parser t)
+  (phi:
+    (b1: bytes) ->
+    (b2: bytes) ->
+    Lemma
+    (requires (injective_precond p b1 b2))
+    (ensures (injective_postcond p b1 b2))
+  )
+: Lemma
+  (injective p)
+= classical_forall_intro_2_requires phi
+
+let no_lookahead_intro
+  (#t: Type)
+  (p: bare_parser t)
+  (phi:
+    (b1: bytes) ->
+    (b2: bytes) ->
+    Lemma
+    (requires (no_lookahead_on_precond p b1 b2))
+    (ensures (no_lookahead_on_postcond p b1 b2))
+  )
+: Lemma
+  (no_lookahead p)
+= classical_forall_intro_2_requires phi
+
+unfold
+let parser_kind_prop0 (#t: Type) (k: parser_kind) (f: bare_parser t) : GTot Type0 =
+  injective f /\
+  (Some? k.parser_kind_subkind ==> parser_subkind_prop (Some?.v k.parser_kind_subkind) f) /\
+  parses_at_least k.parser_kind_low f /\
+  (Some? k.parser_kind_high ==> (parses_at_most (Some?.v k.parser_kind_high) f)) /\
+  parser_kind_metadata_prop k f
+
+let parser_intro
+  (typ : Type0)
+  (spec_parser : P.spec_parser typ)
+  (spec_serializer : P.spec_serializer spec_parser)
+  (spec_parser_injective : (b1: bytes) -> (b2: bytes) -> Lemma
+    (requires (match spec_parser b1, spec_parser b2 with
+    | Some (v1, n1), Some (v2, n2) -> v1 == v2
+    | _ -> False
+    ))
+    (ensures (match spec_parser b1, spec_parser b2 with
+    | Some (v1, n1), Some (v2, n2) -> (n1 <: nat) == n2 /\ Seq.slice b1 0 n1 == Seq.slice b2 0 n2
+    | _ -> True
+  )))
+  (spec_parser_strong_prefix: (b1: bytes) -> (b2: bytes) -> Lemma
+    (requires (
+      match spec_parser b1 with
+      | Some (_, n1) -> n1 <= Seq.length b2 /\ Seq.slice b1 0 n1 == Seq.slice b2 0 n1
+      | _ -> False
+    ))
+    (ensures (
+      match spec_parser b1, spec_parser b2 with
+      | Some (v1, _), Some (v2, _) -> v1 == v2
+      | _ -> False
+  )))
+  (lo: nat)
+  (hi: nat { lo <= hi })
+  (serialized_length : (v:typ) ->
+    Lemma (let l = Seq.length (spec_serializer v) in lo <= l /\ l <= hi))
+: Lemma
+  (parser_kind_prop (strong_parser_kind lo hi None) spec_parser)
+=
+  let parser_bounds (b: bytes) : Lemma
+  (match spec_parser b with
+  | None -> True
+  | Some (_, l) -> lo <= l /\ l <= hi)
+= match spec_parser b with
+  | None -> ()
+  | Some (x, l) ->
+    spec_parser_injective b (spec_serializer x);
+    serialized_length x
+  in
+  parser_injective_intro spec_parser (fun b1 b2 -> spec_parser_injective b1 b2);
+  no_lookahead_intro spec_parser (fun b1 b2 ->
+    spec_parser_strong_prefix b1 b2;
+    spec_parser_injective b1 b2
+  );
+  Classical.forall_intro parser_bounds;
+  assert (parser_kind_prop0 (strong_parser_kind lo hi None) spec_parser);
+  LowParse.Spec.Base.parser_kind_prop_equiv (strong_parser_kind lo hi None) spec_parser
